feat: add proof-of-concept SignedDH example

Chamelean/Label.lean
@@ -23,11 +23,15 @@ def Label.make (l: LabelCtor): Label := {
 def Label.isCorrupt (l: Label) (tr: Trace α) :=
   l.isCorrupt_ (Functor.mapConst () tr)
 
+@[simp, grind]
+theorem Label.makeIsCorrupt (ctor: LabelCtor) (tr: Trace α): (Label.make ctor).isCorrupt tr = ctor.isCorrupt (Functor.mapConst () tr) := by
+  simp [Label.make, isCorrupt]
+
 @[scoped grind→]
-theorem _root_.Chamelean.Trace.MonotoneLemmas.isCorruptLater (l: Label) (tr1 tr2: Trace α):
+theorem _root_.Chamelean.Trace.MonotoneLemmas.isCorrupt_Later (l: Label) (tr1 tr2: Trace Unit):
   tr1 ≤ tr2 →
-  l.isCorrupt tr1 →
-  l.isCorrupt tr2
+  l.isCorrupt_ tr1 →
+  l.isCorrupt_ tr2
   := by
     intro h_le
     induction h_le with
@@ -35,9 +39,20 @@ theorem _root_.Chamelean.Trace.MonotoneLemmas.isCorruptLater (l: Label) (tr1 tr2
     | extend tr2 e h_le ih =>
       intro
       apply l.isCorruptSnoc_
-      suffices l.isCorrupt tr2 by -- ugh
-        simp_all [Label.isCorrupt, map_const, Functor.map] -- uggh
       grind
+
+@[scoped grind→]
+theorem _root_.Chamelean.Trace.MonotoneLemmas.isCorruptLater (l: Label) (tr1 tr2: Trace α):
+  tr1 ≤ tr2 →
+  l.isCorrupt tr1 →
+  l.isCorrupt tr2
+  := by
+    unfold Label.isCorrupt
+    simp only [map_const, Function.comp_apply]
+    intro
+    apply _root_.Chamelean.Trace.MonotoneLemmas.isCorrupt_Later
+    apply Trace.trace_le_map (Function.const α ()) tr1 tr2
+    assumption
 
 def Label.canFlow (l1: Label) (l2: Label) (tr: Trace α): Prop :=
   ∀ trLater,
@@ -53,24 +68,94 @@ theorem _root_.Chamelean.Trace.MonotoneLemmas.canFlowLater (l1: Label) (l2: Labe
     unfold Label.canFlow
     grind [Trace.trace_le_trans]
 
+@[grind]
+theorem canFlowRefl (l: Label) (tr: Trace α):
+  l.canFlow l tr
+  := by
+    unfold Label.canFlow
+    grind
+
+-- @[grind]
+theorem canFlowTrans (l1: Label) (l2: Label) (l3: Label) (tr: Trace α):
+  l1.canFlow l2 tr →
+  l2.canFlow l3 tr →
+  l1.canFlow l3 tr
+  := by
+    unfold Label.canFlow
+    grind
+
 def Label.pub : Label := Label.make {
   isCorrupt tr := True
   isCorruptLater := by grind
 }
+
+@[simp, grind]
+theorem Label.pubIsCorrupt (tr: Trace α): Label.pub.isCorrupt tr := by
+  grind [Label.pub]
+
+@[grind =_]
+theorem canFlowPubEqIsCorrupt (l: Label) (tr: Trace α):
+  l.isCorrupt tr = l.canFlow Label.pub tr
+  := by
+  -- TODO: open doesn't work?
+  -- open Chamelean.Trace.MonotoneLemmas in
+  grind [Label.canFlow, Chamelean.Trace.MonotoneLemmas.isCorruptLater]
 
 def Label.secret : Label := Label.make {
   isCorrupt tr := False
   isCorruptLater := by grind
 }
 
+@[simp, grind]
+theorem Label.secretIsCorrupt (tr: Trace α): ¬ Label.secret.isCorrupt tr := by
+  grind [secret]
+
+@[grind]
+theorem Label.secret.canFlow (l: Label) (tr: Trace α):
+  l.canFlow secret tr
+  := by
+  grind [Label.canFlow]
+
 def Label.join (l1 l2: Label): Label := Label.make {
-  isCorrupt tr := l1.isCorrupt tr ∨ l2.isCorrupt tr
+  isCorrupt tr := l1.isCorrupt_ tr ∨ l2.isCorrupt_ tr
   isCorruptLater := by grind
 }
 
+@[simp, grind]
+theorem Label.joinIsCorrupt (l1 l2: Label) (tr: Trace α):
+  (l1.join l2).isCorrupt tr = (l1.isCorrupt tr ∨ l2.isCorrupt tr)
+  := by
+  grind [join, isCorrupt]
+
 def Label.meet (l1 l2: Label): Label := Label.make {
-  isCorrupt tr := l1.isCorrupt tr ∧ l2.isCorrupt tr
+  isCorrupt tr := l1.isCorrupt_ tr ∧ l2.isCorrupt_ tr
   isCorruptLater := by grind
 }
+
+@[simp, grind]
+theorem Label.meetIsCorrupt (l1 l2: Label) (tr: Trace α):
+  (l1.meet l2).isCorrupt tr = (l1.isCorrupt tr ∧ l2.isCorrupt tr)
+  := by
+  grind [meet, isCorrupt]
+
+@[grind =]
+theorem Label.joinEq (l1: Label) (l2: Label) (l3: Label) (tr: Trace α):
+  l1.canFlow (l2.join l3) tr = (l1.canFlow l2 tr ∧ l1.canFlow l3 tr)
+  := by
+  grind [canFlow]
+
+@[grind]
+theorem Label.joinCanFlowLeft (l1: Label) (l2: Label) (tr: Trace α):
+  (l1.join l2).canFlow l1 tr
+  := by
+  have := joinEq (l1.join l2) l1 l2 tr
+  grind
+
+@[grind]
+theorem Label.joinCanFlowRight (l1: Label) (l2: Label) (tr: Trace α):
+  (l1.join l2).canFlow l2 tr
+  := by
+  have := joinEq (l1.join l2) l1 l2 tr
+  grind
 
 end Chamelean
