Chamelean/SignedDH.lean
@@ -1,0 +1,831 @@
+import Chamelean.Trace
+import Chamelean.Step
+
+open Chamelean
+
+def pure_invariants (x: a) (pre: ProofTrace → Prop) (post: a → ProofTrace → Prop) :=
+  ∀ tr,
+    pre tr → post x tr
+
+theorem apply_pure_invariant
+  {pre: ProofTrace → Prop} {post: a → ProofTrace → Prop}
+  (x: a) (tr: ProofTrace)
+  (inv: pure_invariants x pre post) (p: pre tr):
+  post x tr
+  := inv tr p
+
+instance:
+  HoareTriple
+    (pure x: Traceful a)
+    (fun _ => True)
+    (fun res _ => res = x)
+  where
+    pf := sorry
+
+instance:
+  HoareTriple
+    (OptionT.fail: Traceful a)
+    (fun _ => True)
+    (fun _ _ => True)
+  where
+    pf := sorry
+
+def Principal := String
+def Usage := Principal -- TODO: real type + injectivity
+
+axiom has_usage: Bytes → Usage → ProofTrace → Prop
+
+axiom _root_.Chamelean.Trace.MonotoneLemmas.has_usage_later (b:Bytes) (usg: Usage) (tr1 tr2: ProofTrace): b.invariant tr1 → tr1 ≤ tr2 → has_usage b usg tr1 → has_usage b usg tr2
+
+-- TODO scoped
+grind_pattern _root_.Chamelean.Trace.MonotoneLemmas.has_usage_later =>
+  b.invariant tr1, tr1 ≤ tr2, has_usage b usg tr1
+
+class ParseableSerializeable (a: Type) where
+  parse: Bytes -> Err a
+  serialize: a -> Bytes
+
+  parse_serialize_inv:
+    ∀ x: a,
+      parse (serialize x) = some x
+
+  serialize_parse_inv:
+    ∀ buf: Bytes, ∀ x: a,
+      parse buf = some x →
+      buf = serialize x
+
+open ParseableSerializeable
+
+@[simp, grind =]
+theorem parse_serialize_inv_grind [ParseableSerializeable a] (x: a):
+  ParseableSerializeable.parse (serialize x) = some x
+  := by
+  exact (parse_serialize_inv x)
+
+def formatRel [ParseableSerializeable a] (buf: Bytes) (x: a) :=
+  buf = serialize x
+
+instance [ParseableSerializeable a]:
+  HoareTriple
+    (parse buf: Err a)
+    (fun _ => True)
+    (fun res _ => formatRel buf res)
+where
+  pf := by
+    simp only [hoareTriple, wp, formatRel, OptionT.run]
+    grind [serialize_parse_inv]
+
+theorem serialize_formatRel [ParseableSerializeable a] (x: a):
+  (formatRel (serialize x) x)
+  := by
+    simp [formatRel]
+
+grind_pattern serialize_formatRel => serialize x
+
+def isWellFormed [ParseableSerializeable a] (pre: Bytes → τ → Prop) (x: a) (tr: τ): Prop :=
+  pre (serialize x) tr
+
+theorem isWellFormedFormatRel [ParseableSerializeable a] (pre: Bytes → τ → Prop) (buf: Bytes) (x: a) (tr: τ):
+  formatRel buf x →
+  (pre buf tr = isWellFormed pre x tr)
+  := by
+    grind [isWellFormed, formatRel]
+
+theorem isWellFormedFormatRelBytesInvariant [ParseableSerializeable a]:
+  ∀ (buf: Bytes) (x: a) (tr: ProofTrace),
+  formatRel buf x →
+  (buf.invariant tr = isWellFormed Bytes.invariant x tr)
+  := isWellFormedFormatRel Bytes.invariant
+
+grind_pattern isWellFormedFormatRelBytesInvariant => formatRel buf x, buf.invariant tr
+
+theorem isWellFormedFormatRelIsPublishable [ParseableSerializeable a]:
+  ∀ (buf: Bytes) (x: a) (tr: ProofTrace),
+  formatRel buf x →
+  (buf.is_publishable tr = isWellFormed Bytes.is_publishable x tr)
+  := isWellFormedFormatRel Bytes.is_publishable
+
+grind_pattern isWellFormedFormatRelIsPublishable => formatRel buf x, Bytes.is_publishable buf tr
+
+theorem isWellFormedParse [ParseableSerializeable a] (pre: Bytes → τ → Prop) (buf: Bytes) (x: a) (tr: τ):
+  parse buf = some x →
+  pre buf tr →
+  isWellFormed pre x tr
+  := by
+    grind [isWellFormed, serialize_parse_inv]
+
+class BytesCompatible (pre: Bytes → τ → Prop) where
+  dummy: Unit
+
+instance: BytesCompatible Bytes.invariant where
+  dummy := ()
+
+instance: BytesCompatible is_publishable where
+  dummy := ()
+
+inductive ClientState where
+  | ClientInitiateState (x_sk: Bytes)
+  | ClientFinishState (k_c: Bytes)
+
+instance : ParseableSerializeable ClientState := sorry
+
+inductive ServerState where
+  | ServerFinishState (k_s: Bytes)
+
+instance : ParseableSerializeable ServerState := sorry
+
+structure ClientMessage where
+  x_pk: Bytes
+
+instance : ParseableSerializeable ClientMessage := sorry
+
+@[grind]
+axiom ClientMessage.isWellFormedLemma
+  (pre: Bytes → τ → Prop) [BytesCompatible pre] (x: ClientMessage) (tr: τ):
+  isWellFormed pre x tr = pre x.x_pk tr
+
+structure ServerMessage where
+  y_pk: Bytes
+  sig: Bytes
+
+instance : ParseableSerializeable ServerMessage := sorry
+
+@[grind]
+axiom ServerMessage.isWellFormedLemma
+  (pre: Bytes → τ → Prop) [BytesCompatible pre] (x: ServerMessage) (tr: τ):
+  isWellFormed pre x tr = (
+    pre x.y_pk tr ∧
+    pre x.sig tr
+  )
+
+structure SigInput where
+  x_pk: Bytes
+  y_pk: Bytes
+
+instance : ParseableSerializeable SigInput := sorry
+
+@[grind]
+axiom SigInput.isWellFormedLemma
+  (pre: Bytes → τ → Prop) [BytesCompatible pre] (x: SigInput) (tr: τ):
+  isWellFormed pre x tr = (
+    pre x.x_pk tr ∧
+    pre x.y_pk tr
+  )
+
+inductive SignedDHEvent where
+  | ClientInitiateEvent (x_pk: Bytes)
+  | ServerFinishEvent (x_pk: Bytes) (y_pk: Bytes) (k_s: Bytes)
+  | ClientFinishEvent (server: Principal) (x_pk: Bytes) (y_pk: Bytes) (k_c: Bytes)
+
+instance : ParseableSerializeable SignedDHEvent := sorry
+
+-- setup
+
+def Chamelean.Trace.prefix (tr: Trace α) (i: Nat): Trace α := sorry
+axiom prefix_le (tr: Trace α) (i: Nat): (tr.prefix i) ≤ tr
+grind_pattern prefix_le => tr.prefix i
+
+axiom event_logged_at (who: Principal) (ev: SignedDHEvent) (i: Nat) (tr: ProofTrace): Prop
+abbrev event_logged (who: Principal) (ev: SignedDHEvent) (tr: ProofTrace) :=
+  ∃ i, event_logged_at who ev i tr
+
+namespace Chamelean -- ???
+@[scoped grind→]
+axiom _root_.Chamelean.Trace.MonotoneLemmas.event_logged_at_later (who: Principal) (ev: SignedDHEvent) (i: Nat) (tr1 tr2: ProofTrace): tr1 ≤ tr2 → event_logged_at who ev i tr1 → event_logged_at who ev i tr2
+end Chamelean
+
+def dh_pk (sk: Bytes): Bytes := sorry
+def dh (sk: Bytes) (pk: Bytes): Bytes := sorry
+def vk (sk: Bytes): Bytes := sorry
+def sign (sk: Bytes) (nonce: Bytes) (msg: Bytes): Bytes := sorry
+def verify (vk: Bytes) (msg: Bytes) (sig: Bytes): Bool := sorry
+def hash (b: Bytes): Bytes := sorry
+
+-- invariants
+
+def client_label (me: Principal): Label := sorry
+def server_label (me: Principal): Label := sorry
+def long_term_label (me: Principal): Label := sorry
+
+def sign_pred (sk_usg: Usage) (vk: Bytes) (msg: Bytes) (tr: ProofTrace) :=
+  ∃ server, server = sk_usg ∧ (
+    match parse msg with
+    | none => False
+    | some (msg: SigInput) => (
+      ∃ y_sk,
+        msg.y_pk = dh_pk y_sk ∧
+        y_sk.label tr = server_label server ∧
+        event_logged server (.ServerFinishEvent msg.x_pk msg.y_pk (hash (dh y_sk msg.x_pk))) tr
+    )
+  )
+
+namespace Chamelean -- ???
+@[scoped grind→]
+-- to prove using well-formedness condition that is not yet formalized
+axiom _root_.Chamelean.Trace.MonotoneLemmas.sign_pred_later (sk_usg: Usage) (vk: Bytes) (msg: Bytes) (tr1 tr2: ProofTrace): tr1 ≤ tr2 → sign_pred sk_usg vk msg tr1 → sign_pred sk_usg vk msg tr2
+end Chamelean
+
+def client_state_inv (me: Principal) (sid: Nat) (st: ClientState) (tr: ProofTrace) :=
+  match st with
+  | .ClientInitiateState x_sk =>
+    x_sk.invariant tr ∧
+    x_sk.label tr = client_label me ∧
+    True -- usage
+  | .ClientFinishState k_c =>
+    k_c.invariant tr ∧
+    (k_c.label tr).canFlow (client_label me) tr
+
+namespace Chamelean -- ???
+-- scoped ??
+@[scoped grind→]
+theorem _root_.Chamelean.Trace.MonotoneLemmas.client_state_inv_later
+  (me: Principal) (sid: Nat) (st: ClientState) (tr1 tr2: ProofTrace):
+  tr1 ≤ tr2 → client_state_inv me sid st tr1 → client_state_inv me sid st tr2
+  := by
+    unfold client_state_inv
+    grind
+end Chamelean
+
+
+def server_state_inv (me: Principal) (sid: Nat)(st: ServerState) (tr: ProofTrace) :=
+  match st with
+  | .ServerFinishState k_s =>
+    k_s.invariant tr ∧
+    (k_s.label tr).canFlow (server_label me) tr
+
+instance:
+  HoareTriplePure
+    (dh_pk sk)
+    (fun tr => sk.invariant tr)
+    (fun res tr =>
+      res.invariant tr ∧
+      res.label tr = Label.pub
+      -- and usage
+    )
+  where
+    pf := sorry
+
+def get_dh_label (pk: Bytes) (tr: ProofTrace): Label := sorry
+
+@[grind =]
+theorem get_dh_label_lemma (sk: Bytes) (tr: ProofTrace):
+  get_dh_label (dh_pk sk) tr = sk.label tr
+  := by sorry
+
+axiom _root_.Chamelean.Trace.MonotoneLemmas.get_dh_label_later (b:Bytes) (tr1 tr2: ProofTrace): b.invariant tr1 → tr1 ≤ tr2 → get_dh_label b tr1 = get_dh_label b tr2
+
+axiom dh_eq (sk1 sk2: Bytes): dh sk1 (dh_pk sk2) = dh sk2 (dh_pk sk1)
+grind_pattern dh_eq => dh sk1 (dh_pk sk2), dh sk2 (dh_pk sk1)
+
+-- TODO scoped
+grind_pattern _root_.Chamelean.Trace.MonotoneLemmas.get_dh_label_later =>
+  b.invariant tr1, tr1 ≤ tr2, get_dh_label b tr1
+
+instance:
+  HoareTriplePure
+    (dh sk pk)
+    (fun tr =>
+      sk.invariant tr ∧
+      pk.is_publishable tr
+      -- and usage
+    )
+    (fun res tr =>
+      res.invariant tr ∧
+      res.label tr = Label.join (sk.label tr) (get_dh_label pk tr)
+      -- and usage
+    )
+  where
+    pf := sorry
+
+axiom vk_spec (sk: Bytes):
+  pure_invariants (vk sk)
+  (fun tr =>
+    sk.invariant tr
+  )
+  (fun res tr =>
+    res.invariant tr ∧
+    res.label tr = Label.pub
+    -- and usage
+  )
+
+def get_sign_label (vk: Bytes) (tr: ProofTrace): Label := sorry
+axiom get_sign_label_lemma (sk: Bytes) (tr: ProofTrace):
+  sk.label tr = get_sign_label (vk sk) tr
+
+axiom _root_.Chamelean.Trace.MonotoneLemmas.get_sign_label_later (b:Bytes) (tr1 tr2: ProofTrace): b.invariant tr1 → tr1 ≤ tr2 → get_sign_label b tr1 = get_sign_label b tr2
+
+-- TODO scoped
+grind_pattern _root_.Chamelean.Trace.MonotoneLemmas.get_sign_label_later =>
+  b.invariant tr1, tr1 ≤ tr2, get_sign_label b tr1
+
+def has_sign_usage (vk: Bytes) (usg: Usage) (tr: ProofTrace): Prop := sorry
+axiom has_sign_usage_lemma (sk: Bytes) (usg: Usage) (tr: ProofTrace):
+  has_usage sk usg tr = has_sign_usage (vk sk) usg tr
+
+axiom _root_.Chamelean.Trace.MonotoneLemmas.has_sign_usage_later (b:Bytes) (usg: Usage) (tr1 tr2: ProofTrace): b.invariant tr1 → tr1 ≤ tr2 → has_sign_usage b usg tr1 → has_sign_usage b usg tr2
+
+-- TODO scoped
+grind_pattern _root_.Chamelean.Trace.MonotoneLemmas.has_sign_usage_later =>
+  b.invariant tr1, tr1 ≤ tr2, has_sign_usage b usg tr1
+
+instance: HasGhostArgumentType (sign sk nonce msg) Usage
+where
+  dummy := ()
+
+def signMetaprog: GhostParameterFinder where
+  findGhost mvar e :=
+  Lean.withTraceNode `Step (fun _ => pure m!"signMetaprog") do
+    let sk_mvar ← Lean.Meta.mkFreshExprMVar (some (.const ``Bytes []))
+    let nonce_mvar ← Lean.Meta.mkFreshExprMVar (some (.const ``Bytes []))
+    let msg_mvar ← Lean.Meta.mkFreshExprMVar (some (.const ``Bytes []))
+    let signToUnify ← Lean.Meta.mkAppM ``sign #[sk_mvar, nonce_mvar, msg_mvar]
+    trace[Step] "gonna unify {e} and {signToUnify}"
+    unless ← Lean.Meta.isDefEq e signToUnify do
+      throwError "signMetaprog: cannot unify {e} and {signToUnify}"
+    trace[Step] "got {signToUnify}"
+
+    let usg_mvar := .mvar mvar
+    let tr_mvar ← Lean.Meta.mkFreshExprMVar (some (.const ``ProofTrace []))
+    let hasUsageToUnify ← Lean.Meta.mkAppM ``has_usage #[sk_mvar, usg_mvar, tr_mvar]
+    trace[Step] "gonna find {hasUsageToUnify} in assumptions"
+    let .mvar hasUsageMvar ← Lean.Meta.mkFreshExprMVar hasUsageToUnify
+      | throwError ""
+    hasUsageMvar.assumption
+
+instance: HasGhostMetaprogram (sign sk nonce msg) signMetaprog
+where
+  dummy := ()
+
+instance:
+  HoareTriplePureGhost
+    (sign sk nonce msg)
+    (sk_usg)
+    (fun tr =>
+      sk.invariant tr ∧
+      nonce.invariant tr ∧
+      msg.invariant tr ∧
+      has_usage sk sk_usg tr ∧
+      -- nonce usage
+      (sk.label tr).canFlow (nonce.label tr) tr ∧ (
+        (
+          -- sk usage
+          sign_pred sk_usg (vk sk) msg tr
+        ) ∨ (
+          (sk.label tr).canFlow Label.pub tr
+        )
+      )
+    )
+    (fun res tr =>
+      res.invariant tr ∧
+      res.label tr = msg.label tr
+    )
+  where
+    pf := sorry
+
+instance: HasGhostArgumentType (verify vkey msg sig) Usage
+where
+  dummy := ()
+
+def verifyMetaprog: GhostParameterFinder where
+  findGhost mvar e :=
+  Lean.withTraceNode `Step (fun _ => pure m!"verifyMetaprog") do
+    let vkey_mvar ← Lean.Meta.mkFreshExprMVar (some (.const ``Bytes []))
+    let msg_mvar ← Lean.Meta.mkFreshExprMVar (some (.const ``Bytes []))
+    let sig_mvar ← Lean.Meta.mkFreshExprMVar (some (.const ``Bytes []))
+    let verifyToUnify ← Lean.Meta.mkAppM ``verify #[vkey_mvar, msg_mvar, sig_mvar]
+    trace[Step] "gonna unify {e} and {verifyToUnify}"
+    unless ← Lean.Meta.isDefEq e verifyToUnify do
+      throwError "verifyMetaprog: cannot unify {e} and {verifyToUnify}"
+    trace[Step] "got {verifyToUnify}"
+
+    let usg_mvar := .mvar mvar
+    let tr_mvar ← Lean.Meta.mkFreshExprMVar (some (.const ``ProofTrace []))
+    let hasUsageToUnify ← Lean.Meta.mkAppM ``has_sign_usage #[vkey_mvar, usg_mvar, tr_mvar]
+    trace[Step] "gonna find {hasUsageToUnify} in assumptions"
+    let .mvar hasUsageMvar ← Lean.Meta.mkFreshExprMVar hasUsageToUnify
+      | throwError ""
+    hasUsageMvar.assumption
+
+instance: HasGhostMetaprogram (verify vkey msg sig) verifyMetaprog
+where
+  dummy := ()
+
+instance:
+  HoareTriplePureGhost
+    (verify vkey msg sig)
+    (sk_usg: Usage)
+    (fun tr =>
+      vkey.invariant tr ∧
+      msg.invariant tr ∧
+      sig.invariant tr ∧
+      has_sign_usage vkey sk_usg tr
+    )
+    (fun res tr =>
+      res → (
+        (
+          --usage
+          sign_pred sk_usg vkey msg tr
+        ) ∨ (
+          (get_sign_label vkey tr).canFlow Label.pub tr
+        )
+      )
+    )
+  where
+    pf := sorry
+
+instance:
+  HoareTriplePure
+    (hash b)
+    (fun tr => b.invariant tr)
+    (fun res tr =>
+      res.invariant tr ∧
+      res.label tr = b.label tr
+    )
+  where
+    pf := sorry
+
+def gen_rand (len: Nat) : Traceful Bytes := sorry
+def send_message (b:Bytes) : Traceful Nat := sorry
+def receive_message (ts: Nat): Traceful Bytes := sorry
+def new_sid (me: Principal): Traceful Nat := sorry
+def set_client_state (me: Principal) (sid: Nat) (st: ClientState): Traceful Unit := sorry
+def get_client_state (me: Principal) (sid: Nat): Traceful ClientState  := sorry
+def set_server_state (me: Principal) (sid: Nat) (st: ServerState): Traceful Unit := sorry
+def get_server_state (me: Principal) (sid: Nat): Traceful ServerState  := sorry
+def get_public_key (who: Principal): Traceful Bytes := sorry
+def get_private_key (who: Principal): Traceful Bytes := sorry
+def log_event (who: Principal) (ev: SignedDHEvent): Traceful Unit := sorry
+
+instance: HasGhostArgumentType (gen_rand len) Label
+where
+  dummy := ()
+
+instance:
+  HoareTripleGhost
+    (gen_rand len)
+    lab
+    (fun _ => True)
+    (fun b tr =>
+      b.invariant tr ∧
+      b.label tr = lab
+      -- usage, length
+    )
+  where
+    pf := sorry
+
+instance:
+  HoareTriple
+    (send_message b)
+    (fun tr => b.is_publishable tr)
+    (fun _ _ => True)
+  where
+    pf := sorry
+
+instance:
+  HoareTriple
+    (receive_message ts)
+    (fun _ => True)
+    (fun b tr => b.is_publishable tr)
+  where
+    pf := sorry
+
+instance:
+  HoareTriple
+    (new_sid me)
+    (fun _ => True)
+    (fun _ _ => True)
+  where
+    pf := sorry
+
+instance:
+  HoareTriple
+    (set_client_state me sid st)
+    (fun tr => client_state_inv me sid st tr)
+    (fun _ _ => True)
+  where
+    pf := sorry
+
+instance:
+  HoareTriple
+    (get_client_state me sid)
+    (fun _ => True)
+    (fun st tr => client_state_inv me sid st tr)
+  where
+    pf := sorry
+
+instance:
+  HoareTriple
+    (set_server_state me sid st)
+    (fun tr => server_state_inv me sid st tr)
+    (fun _ _ => True)
+  where
+    pf := sorry
+
+instance:
+  HoareTriple
+    (get_server_state me sid)
+    (fun _ => True)
+    (fun st tr => server_state_inv me sid st tr)
+  where
+    pf := sorry
+
+instance:
+  HoareTriple
+    (get_public_key who)
+    (fun _ => True)
+    (fun vk tr =>
+      vk.invariant tr ∧
+      get_sign_label vk tr = long_term_label who ∧
+      has_sign_usage vk who tr
+    )
+  where
+    pf := sorry
+
+instance:
+  HoareTriple
+    (get_private_key who)
+    (fun _ => True)
+    (fun sk tr =>
+      sk.invariant tr ∧
+      sk.label tr = long_term_label who ∧
+      has_usage sk who tr
+    )
+  where
+    pf := sorry
+
+def event_pred (me: Principal) (ev: SignedDHEvent) (tr: ProofTrace) :=
+  match ev with
+  | .ClientInitiateEvent x_pk => (
+    x_pk.invariant tr ∧
+    get_dh_label x_pk tr = client_label me
+  )
+  | .ServerFinishEvent x_pk _y_pk k_s => (
+    k_s.invariant tr ∧
+    x_pk.invariant tr ∧
+    k_s.label tr = (server_label me).join (get_dh_label x_pk tr)
+  )
+  | .ClientFinishEvent server x_pk y_pk k_c => (
+    (
+      event_logged server (.ServerFinishEvent x_pk y_pk k_c) tr ∧
+      k_c.invariant tr ∧
+      k_c.label tr = (client_label me).join (server_label server)
+    ) ∨ (long_term_label server).isCorrupt tr
+  )
+
+instance:
+  HoareTriple
+    (log_event who ev)
+    (fun tr => event_pred who ev tr)
+    (fun () tr => event_logged who ev tr)
+  where
+    pf := sorry
+
+@[grind→]
+axiom event_logged_at_implies_event_pred
+  (who: Principal) (ev: SignedDHEvent) (i: Nat) (tr: ProofTrace):
+    event_logged_at who ev i tr →
+    tr.invariant →
+    event_pred who ev (tr.prefix i)
+
+-- signed dh
+
+namespace SignedDH
+
+def client_initiate (me: Principal): Traceful (Nat × Nat) := do
+  let x_sk ← gen_rand 32
+  let x_pk := dh_pk x_sk
+
+  log_event me (.ClientInitiateEvent x_pk)
+  let sid ← new_sid me
+  set_client_state me sid (.ClientInitiateState x_sk)
+  let msg_ts ← send_message (serialize ({ x_pk } : ClientMessage))
+  pure (sid, msg_ts)
+
+def server_receive (me: Principal) (msg_ts: Nat) : Traceful (Nat × Nat) := do
+  let msg_bytes ← receive_message msg_ts
+  let msg: ClientMessage ← parse msg_bytes
+  let x_pk := msg.x_pk
+  let my_sig_key ← get_private_key me
+
+  let y_sk ← gen_rand 32
+  let y_pk := dh_pk y_sk
+  let k_s := hash (dh y_sk x_pk)
+  let sig_nonce ← gen_rand 32
+  let sig := sign my_sig_key sig_nonce (serialize ({x_pk, y_pk}: SigInput))
+
+  log_event me (.ServerFinishEvent x_pk y_pk k_s)
+  let sid ← new_sid me
+  set_server_state me sid (.ServerFinishState k_s)
+  let msg_ts ← send_message (serialize ({ y_pk, sig } : ServerMessage))
+  pure (sid, msg_ts)
+
+def client_finish (me: Principal) (server: Principal) (msg_ts: Nat) (sid: Nat) : Traceful Unit := do
+  let msg_bytes ← receive_message msg_ts
+  let msg: ServerMessage ← parse msg_bytes
+
+  let my_state ← get_client_state me sid
+  let .ClientInitiateState x_sk := my_state
+    | OptionT.fail
+
+  let server_vk ← get_public_key server
+
+  let x_pk := dh_pk x_sk
+  guard (verify server_vk (serialize ({ x_pk, y_pk := msg.y_pk }: SigInput)) msg.sig)
+  let k_c := hash (dh x_sk msg.y_pk)
+
+  log_event me (.ClientFinishEvent server x_pk msg.y_pk k_c)
+  set_client_state me sid (.ClientFinishState k_c)
+
+instance:
+  HoareTriple
+    (client_initiate me)
+    (fun _ => True)
+    (fun _ _ => True)
+where
+  pf := by
+    unfold client_initiate
+    step with ⟨ client_label me ⟩
+    step
+    step by grind [event_pred]
+    step
+    step by grind [client_state_inv]
+    step
+    step
+    grind
+
+instance:
+  HoareTriple
+    (server_receive me msg_ts)
+    (fun _ => True)
+    (fun _ _ => True)
+where
+  pf := by
+    unfold server_receive
+    step
+    step
+    step_intro
+    step
+    step with ⟨ server_label me ⟩
+    step
+    hoist
+    step
+    step
+    step with ⟨ Label.secret ⟩
+    hoist
+    step_intro
+    -- for monotonicity TODO: how to infer is_publishable automatically?
+    have h_sig_msg: sig_msg.is_publishable tr := by grind
+    -- interesting stuff: we will prove things on `sig` later on,
+    -- because we need to log the event before
+    step_intro
+    step by grind [event_pred]
+    step_let sig with ⟨ me ⟩ by grind [sign_pred]
+    step
+    step by grind [server_state_inv]
+    step
+    step
+    grind
+
+instance:
+  HoareTriple
+    (client_finish me server msg_ts sid)
+    (fun _ => True)
+    (fun _ _ => True)
+where
+  pf := by
+    unfold client_finish
+    step
+    step
+    step
+    split
+    case h_1 x_sk h_x_sk =>
+      -- this is useful to monotonize hypothesis
+      -- (probably best as a grind pattern on client_state_inv but well)
+      have h_x_sk': x_sk.invariant tr := by grind [client_state_inv]
+      step
+      step
+      step with ⟨ server ⟩
+      hoist
+      step
+      step
+      step by grind [event_pred, sign_pred, client_state_inv]
+      step by grind [client_state_inv]
+      grind
+    · step
+      grind
+
+theorem client_auth:
+  event_logged_at client (.ClientFinishEvent server x_pk y_pk k) time tr →
+  tr.invariant → (
+    let tr_before := tr.prefix time
+    event_logged server (.ServerFinishEvent x_pk y_pk k) tr_before  ∨
+    (long_term_label server).isCorrupt tr_before
+  )
+  := by
+    intro h_ev h_trinv
+    have := event_logged_at_implies_event_pred _ _ _ _ h_ev h_trinv
+    simp [event_pred] at this
+    grind
+
+theorem client_secrecy:
+  k.is_publishable tr → -- attacker_knows
+  event_logged_at client (.ClientFinishEvent server x_pk y_pk k) time tr →
+  tr.invariant → (
+    let tr_before := tr.prefix time
+    (long_term_label server).isCorrupt tr_before ∨
+    (client_label client).isCorrupt tr ∨
+    (server_label server).isCorrupt tr
+  )
+  := by
+    intro h_pub h_ev h_trinv
+    have h_ev := event_logged_at_implies_event_pred _ _ _ _ h_ev h_trinv
+    simp [event_pred] at h_ev
+    grind
+
+
+namespace TestGrindAnnot
+
+-- Test for a more automatic feeling
+attribute [grind] event_pred
+attribute [grind] client_state_inv
+attribute [grind] server_state_inv
+attribute [grind] sign_pred
+
+instance:
+  HoareTriple
+    (client_initiate me)
+    (fun _ => True)
+    (fun _ _ => True)
+where
+  pf := by
+    unfold client_initiate
+    step with ⟨ client_label me ⟩
+    step
+    step
+    step
+    step
+    step
+    step
+    grind
+
+instance:
+  HoareTriple
+    (server_receive me msg_ts)
+    (fun _ => True)
+    (fun _ _ => True)
+where
+  pf := by
+    unfold server_receive
+    step
+    step
+    step_intro
+    step
+    step with ⟨ server_label me ⟩
+    step
+    hoist
+    step
+    step
+    step with ⟨ Label.secret ⟩
+    hoist
+    step_intro
+    -- for monotonicity TODO: how to infer is_publishable automatically?
+    have h_sig_msg: sig_msg.is_publishable tr := by grind
+    -- interesting stuff: we will prove things on `sig` later on,
+    -- because we need to log the event before
+    step_intro
+    step
+    step_let sig -- with ⟨ me ⟩
+    step
+    step
+    step
+    step
+    grind
+
+instance:
+  HoareTriple
+    (client_finish me server msg_ts sid)
+    (fun _ => True)
+    (fun _ _ => True)
+where
+  pf := by
+    unfold client_finish
+    step
+    step
+    step
+    split
+    case h_1 x_sk h_x_sk =>
+      step
+      step
+      step -- with ⟨ server ⟩
+      hoist
+      step
+      step
+      step
+      step
+      grind
+    · step
+      grind
+
+end TestGrindAnnot
+
+end SignedDH
